

Title Goes Here

Barry Denby

Griffith College Dublin

April 30, 2025

Amdhal's law proof

- ▶ define the meaning of a few terms first
 - ▶ S is speedup
 - ▶ $T(1)$ is the time taken for the serial (1 process/thread) solution
 - ▶ $T(N)$ is the time taken for the parallel solution
 - ▶ α is the proportion of code that is serial
 - ▶ $1 - \alpha$ is the proportion of code that is parallel

Amdhal's law proof

- ▶ Define $S = \frac{1}{\alpha}$
- ▶ Define $T(1) = \sigma + \pi$
- ▶ Define $T(N) = \sigma + \frac{\pi}{N}$
- ▶ Define $\alpha = \frac{\sigma}{\sigma + \pi}$
- ▶ Define $1 - \alpha = \frac{\pi}{\sigma + \pi}$

Amdhal's law proof

- ▶ First speedup is defined as the following
- ▶ $S(N) = \frac{T(1)}{T(N)}$
- ▶ Substitute in for $T(1)$ and $T(N)$ using definitions on previous slide
- ▶ $S(N) = \frac{\sigma + \pi}{\sigma + \frac{\pi}{N}}$

Amdhal's law proof

- ▶ Divide top and bottom by σ
- ▶
$$S(N) = \frac{\frac{\sigma}{\sigma} + \frac{\pi}{\sigma}}{\frac{\sigma}{\sigma} + \frac{\pi}{N\sigma}}$$
- ▶ When we clean it up we get the following
- ▶
$$S(N) = \frac{1 + \frac{\pi}{\sigma}}{1 + \frac{\pi}{N\sigma}}$$
- ▶ however we really don't like the σ and π in there but want α instead so lets define a formula to see if we can find a way to substitute them

Amdhal's law proof

- ▶ $\frac{1-\alpha}{\alpha} = \frac{\frac{\pi}{\sigma+\pi}}{\frac{\sigma}{\sigma+\pi}}$
- ▶ To divide a fraction flip it and multiply
- ▶ $\frac{1-\alpha}{\alpha} = \frac{\pi}{\sigma+\pi} \frac{\sigma+\pi}{\sigma}$
- ▶ the $\sigma + \pi$ cancel out and leave us with
- ▶ $\frac{1-\alpha}{\alpha} = \frac{\pi}{\sigma}$

Amdhal's law proof

- ▶ So now we can swap out the $\frac{\pi}{\sigma}$ for $\frac{1-\alpha}{\alpha}$
- ▶
$$S(N) = \frac{1 + \frac{1-\alpha}{\alpha}}{1 + \frac{1-\alpha}{N\alpha}}$$
- ▶ multiply top and bottom by α to remove the α on the bottom of the fractions
- ▶
$$S(N) = \frac{\alpha + 1 - \alpha}{\alpha + \frac{1-\alpha}{N}}$$

Amdhal's law proof

- ▶ The α and $-\alpha$ on the top line cancel out
- ▶ $S(N) = \frac{1}{\alpha + \frac{1-\alpha}{N}}$
- ▶ Nearly there but that last fraction on the bottom right is a touch annoying. However if we introduce limits we can deal with it
- ▶ $\lim_{N \rightarrow \infty} S(N) = \frac{1}{\alpha + \frac{1-\alpha}{N}} = \frac{1}{\alpha}$

Gustaffson's law proof

- ▶ Define $S = \frac{1}{\alpha}$
- ▶ Define $T(1) = \sigma + N\pi$
- ▶ Define $T(N) = \sigma + \pi$
- ▶ Define $\alpha = \frac{\sigma}{\sigma + \pi}$
- ▶ Define $1 - \alpha = \frac{\pi}{\sigma + \pi}$

Gustaffson's law proof

- ▶ First speedup is defined as the following
- ▶ $S(N) = \frac{T(1)}{T(N)}$
- ▶ Substitute in for $T(1)$ and $T(N)$ using definitions on previous slide
- ▶ $S(N) = \frac{\sigma + N\pi}{\sigma + \pi}$
- ▶ Split out the fraction into its two parts
- ▶ $S(N) = \frac{\sigma}{\sigma + \pi} + \frac{N\pi}{\sigma + \pi}$
- ▶

Gustaffson's law proof

- ▶ The first part of the fraction can be substituted out for α and the second part can mostly be substituted out for $1 - \alpha$
- ▶ $S(N) = \alpha + N(1 - \alpha)$
- ▶ Multiply out the brackets
- ▶ $S(N) = \alpha + N - N\alpha$

Gustaffson's law proof

- ▶ Reorder the terms
- ▶ $S(N) = N - N\alpha + \alpha$
- ▶ factor out $-\alpha$
- ▶ $S(N) = N - \alpha(N - 1)$